arith wip

libcrux-ml-kem/src/vector/portable/ntt.rs
@@ -2,111 +2,119 @@ use super::arithmetic::*;
 use super::vector_type::*;
 
 #[inline(always)]
-pub(crate) fn ntt_step(v: &mut PortableVector, zeta: i16, i: usize, j: usize) {
-    let t = montgomery_multiply_fe_by_fer(v.elements[j], zeta);
-    v.elements[j] = v.elements[i] - t;
-    v.elements[i] = v.elements[i] + t;
+#[hax_lib::requires(fstar!("v i < 16 /\\ v j < 16 /\\ Spec.Utils.is_i16b 1664 $zeta"))]
+pub(crate) fn ntt_step(vec: &mut PortableVector, zeta: i16, i: usize, j: usize) {
+    let t = montgomery_multiply_fe_by_fer(vec.elements[j], zeta);
+    vec.elements[j] = vec.elements[i] - t;
+    vec.elements[i] = vec.elements[i] + t;
 }
 
 #[inline(always)]
+#[hax_lib::requires(fstar!("Spec.Utils.is_i16b 1664 zeta0 /\\ Spec.Utils.is_i16b 1664 zeta1 /\\ Spec.Utils.is_i16b 1664 zeta2 /\\ Spec.Utils.is_i16b 1664 zeta3"))]
 pub(crate) fn ntt_layer_1_step(
-    mut v: PortableVector,
+    mut vec: PortableVector,
     zeta0: i16,
     zeta1: i16,
     zeta2: i16,
     zeta3: i16,
 ) -> PortableVector {
-    ntt_step(&mut v, zeta0, 0, 2);
-    ntt_step(&mut v, zeta0, 1, 3);
-    ntt_step(&mut v, zeta1, 4, 6);
-    ntt_step(&mut v, zeta1, 5, 7);
-    ntt_step(&mut v, zeta2, 8, 10);
-    ntt_step(&mut v, zeta2, 9, 11);
-    ntt_step(&mut v, zeta3, 12, 14);
-    ntt_step(&mut v, zeta3, 13, 15);
-    v
+    ntt_step(&mut vec, zeta0, 0, 2);
+    ntt_step(&mut vec, zeta0, 1, 3);
+    ntt_step(&mut vec, zeta1, 4, 6);
+    ntt_step(&mut vec, zeta1, 5, 7);
+    ntt_step(&mut vec, zeta2, 8, 10);
+    ntt_step(&mut vec, zeta2, 9, 11);
+    ntt_step(&mut vec, zeta3, 12, 14);
+    ntt_step(&mut vec, zeta3, 13, 15);
+    vec
 }
 
 #[inline(always)]
-pub(crate) fn ntt_layer_2_step(mut v: PortableVector, zeta0: i16, zeta1: i16) -> PortableVector {
-    ntt_step(&mut v, zeta0, 0, 4);
-    ntt_step(&mut v, zeta0, 1, 5);
-    ntt_step(&mut v, zeta0, 2, 6);
-    ntt_step(&mut v, zeta0, 3, 7);
-    ntt_step(&mut v, zeta1, 8, 12);
-    ntt_step(&mut v, zeta1, 9, 13);
-    ntt_step(&mut v, zeta1, 10, 14);
-    ntt_step(&mut v, zeta1, 11, 15);
-    v
+#[hax_lib::requires(fstar!("Spec.Utils.is_i16b 1664 zeta0 /\\ Spec.Utils.is_i16b 1664 zeta1"))]
+pub(crate) fn ntt_layer_2_step(mut vec: PortableVector, zeta0: i16, zeta1: i16) -> PortableVector {
+    ntt_step(&mut vec, zeta0, 0, 4);
+    ntt_step(&mut vec, zeta0, 1, 5);
+    ntt_step(&mut vec, zeta0, 2, 6);
+    ntt_step(&mut vec, zeta0, 3, 7);
+    ntt_step(&mut vec, zeta1, 8, 12);
+    ntt_step(&mut vec, zeta1, 9, 13);
+    ntt_step(&mut vec, zeta1, 10, 14);
+    ntt_step(&mut vec, zeta1, 11, 15);
+    vec
 }
 
 #[inline(always)]
-pub(crate) fn ntt_layer_3_step(mut v: PortableVector, zeta: i16) -> PortableVector {
-    ntt_step(&mut v, zeta, 0, 8);
-    ntt_step(&mut v, zeta, 1, 9);
-    ntt_step(&mut v, zeta, 2, 10);
-    ntt_step(&mut v, zeta, 3, 11);
-    ntt_step(&mut v, zeta, 4, 12);
-    ntt_step(&mut v, zeta, 5, 13);
-    ntt_step(&mut v, zeta, 6, 14);
-    ntt_step(&mut v, zeta, 7, 15);
-    v
+#[hax_lib::requires(fstar!("Spec.Utils.is_i16b 1664 zeta"))]
+pub(crate) fn ntt_layer_3_step(mut vec: PortableVector, zeta: i16) -> PortableVector {
+    ntt_step(&mut vec, zeta, 0, 8);
+    ntt_step(&mut vec, zeta, 1, 9);
+    ntt_step(&mut vec, zeta, 2, 10);
+    ntt_step(&mut vec, zeta, 3, 11);
+    ntt_step(&mut vec, zeta, 4, 12);
+    ntt_step(&mut vec, zeta, 5, 13);
+    ntt_step(&mut vec, zeta, 6, 14);
+    ntt_step(&mut vec, zeta, 7, 15);
+    vec
 }
 
 #[inline(always)]
-pub(crate) fn inv_ntt_step(v: &mut PortableVector, zeta: i16, i: usize, j: usize) {
-    let a_minus_b = v.elements[j] - v.elements[i];
-    v.elements[i] = barrett_reduce_element(v.elements[i] + v.elements[j]);
-    v.elements[j] = montgomery_multiply_fe_by_fer(a_minus_b, zeta);
+#[hax_lib::requires(fstar!("v i < 16 /\\ v j < 16 /\\ Spec.Utils.is_i16b 1664 $zeta"))]
+pub(crate) fn inv_ntt_step(vec: &mut PortableVector, zeta: i16, i: usize, j: usize) {
+    let a_minus_b = vec.elements[j] - vec.elements[i];
+    vec.elements[i] = barrett_reduce_element(vec.elements[i] + vec.elements[j]);
+    vec.elements[j] = montgomery_multiply_fe_by_fer(a_minus_b, zeta);
 }
 
 #[inline(always)]
+#[hax_lib::requires(fstar!("Spec.Utils.is_i16b 1664 zeta0 /\\ Spec.Utils.is_i16b 1664 zeta1 /\\ Spec.Utils.is_i16b 1664 zeta2 /\\ Spec.Utils.is_i16b 1664 zeta3"))]
 pub(crate) fn inv_ntt_layer_1_step(
-    mut v: PortableVector,
+    mut vec: PortableVector,
     zeta0: i16,
     zeta1: i16,
     zeta2: i16,
     zeta3: i16,
 ) -> PortableVector {
-    inv_ntt_step(&mut v, zeta0, 0, 2);
-    inv_ntt_step(&mut v, zeta0, 1, 3);
-    inv_ntt_step(&mut v, zeta1, 4, 6);
-    inv_ntt_step(&mut v, zeta1, 5, 7);
-    inv_ntt_step(&mut v, zeta2, 8, 10);
-    inv_ntt_step(&mut v, zeta2, 9, 11);
-    inv_ntt_step(&mut v, zeta3, 12, 14);
-    inv_ntt_step(&mut v, zeta3, 13, 15);
-    v
+    inv_ntt_step(&mut vec, zeta0, 0, 2);
+    inv_ntt_step(&mut vec, zeta0, 1, 3);
+    inv_ntt_step(&mut vec, zeta1, 4, 6);
+    inv_ntt_step(&mut vec, zeta1, 5, 7);
+    inv_ntt_step(&mut vec, zeta2, 8, 10);
+    inv_ntt_step(&mut vec, zeta2, 9, 11);
+    inv_ntt_step(&mut vec, zeta3, 12, 14);
+    inv_ntt_step(&mut vec, zeta3, 13, 15);
+    vec
 }
 
 #[inline(always)]
+#[hax_lib::requires(fstar!("Spec.Utils.is_i16b 1664 zeta0 /\\ Spec.Utils.is_i16b 1664 zeta1"))]
 pub(crate) fn inv_ntt_layer_2_step(
-    mut v: PortableVector,
+    mut vec: PortableVector,
     zeta0: i16,
     zeta1: i16,
 ) -> PortableVector {
-    inv_ntt_step(&mut v, zeta0, 0, 4);
-    inv_ntt_step(&mut v, zeta0, 1, 5);
-    inv_ntt_step(&mut v, zeta0, 2, 6);
-    inv_ntt_step(&mut v, zeta0, 3, 7);
-    inv_ntt_step(&mut v, zeta1, 8, 12);
-    inv_ntt_step(&mut v, zeta1, 9, 13);
-    inv_ntt_step(&mut v, zeta1, 10, 14);
-    inv_ntt_step(&mut v, zeta1, 11, 15);
-    v
+    inv_ntt_step(&mut vec, zeta0, 0, 4);
+    inv_ntt_step(&mut vec, zeta0, 1, 5);
+    inv_ntt_step(&mut vec, zeta0, 2, 6);
+    inv_ntt_step(&mut vec, zeta0, 3, 7);
+    inv_ntt_step(&mut vec, zeta1, 8, 12);
+    inv_ntt_step(&mut vec, zeta1, 9, 13);
+    inv_ntt_step(&mut vec, zeta1, 10, 14);
+    inv_ntt_step(&mut vec, zeta1, 11, 15);
+    vec
 }
 
 #[inline(always)]
-pub(crate) fn inv_ntt_layer_3_step(mut v: PortableVector, zeta: i16) -> PortableVector {
-    inv_ntt_step(&mut v, zeta, 0, 8);
-    inv_ntt_step(&mut v, zeta, 1, 9);
-    inv_ntt_step(&mut v, zeta, 2, 10);
-    inv_ntt_step(&mut v, zeta, 3, 11);
-    inv_ntt_step(&mut v, zeta, 4, 12);
-    inv_ntt_step(&mut v, zeta, 5, 13);
-    inv_ntt_step(&mut v, zeta, 6, 14);
-    inv_ntt_step(&mut v, zeta, 7, 15);
-    v
+#[hax_lib::requires(fstar!("Spec.Utils.is_i16b 1664 zeta"))]
+pub(crate) fn inv_ntt_layer_3_step(mut vec: PortableVector, zeta: i16) -> PortableVector {
+    inv_ntt_step(&mut vec, zeta, 0, 8);
+    inv_ntt_step(&mut vec, zeta, 1, 9);
+    inv_ntt_step(&mut vec, zeta, 2, 10);
+    inv_ntt_step(&mut vec, zeta, 3, 11);
+    inv_ntt_step(&mut vec, zeta, 4, 12);
+    inv_ntt_step(&mut vec, zeta, 5, 13);
+    inv_ntt_step(&mut vec, zeta, 6, 14);
+    inv_ntt_step(&mut vec, zeta, 7, 15);
+    vec
 }
 
 /// Compute the product of two Kyber binomials with respect to the
@@ -130,11 +138,17 @@ pub(crate) fn inv_ntt_layer_3_step(mut v: PortableVector, zeta: i16) -> Portable
 /// The NIST FIPS 203 standard can be found at
 /// <https://csrc.nist.gov/pubs/fips/203/ipd>.
 #[inline(always)]
-#[hax_lib::ensures(|()| fstar!("(Seq.index out_future (v i), Seq.index out_future (v j)) ==
-                        Spec.MLKEM.Math.poly_base_case_multiply 
-                            (Seq.index a (v i)) (Seq.index a (v j))
-                            (Seq.index b (v i)) (Seq.index b (v j))
-                            (v zeta) "))]
+#[hax_lib::requires(fstar!("v i < 16 /\\ v j < 16 /\\ Spec.Utils.is_i16b 1664 $zeta"))]
+#[hax_lib::ensures(|()| fstar!("
+        let (x,y) = 
+          Spec.MLKEM.Math.poly_base_case_multiply 
+            (v (Seq.index a.f_elements (v i)) % 3329)
+            (v (Seq.index a.f_elements (v j)) % 3329)
+            (v (Seq.index b.f_elements (v i)) % 3329)
+            (v (Seq.index b.f_elements (v j)) % 3329)
+            ((v zeta * 169) % 3329) in
+          (x == v (Seq.index out_future.f_elements (v i)) % 3329 /\\
+           y == v (Seq.index out_future.f_elements (v j)) % 3329))"))]
 pub(crate) fn ntt_multiply_binomials(
     a: &PortableVector,
     b: &PortableVector,
@@ -143,11 +157,16 @@ pub(crate) fn ntt_multiply_binomials(
     j: usize,
     out: &mut PortableVector,
 ) {
+    hax_lib::fstar!("Spec.Utils.lemma_mul_i16b 3328 3328 (Seq.index (${a}.f_elements) (v i)) (Seq.index (${b}.f_elements) (v i))");
+    hax_lib::fstar!("Spec.Utils.lemma_mul_i16b 3328 3328 (Seq.index (${a}.f_elements) (v j)) (Seq.index (${b}.f_elements) (v j))");
+    let ai_bi = (a.elements[i] as i32) * (b.elements[i] as i32);
+    let aj_bj = montgomery_reduce_element((a.elements[j] as i32) * (b.elements[j] as i32));
+    hax_lib::fstar!("Spec.Utils.lemma_mul_i16b 3328 1664 $aj_bj $zeta");
     let o0 = montgomery_reduce_element(
-        (a.elements[i] as i32) * (b.elements[i] as i32)
-            + (montgomery_reduce_element((a.elements[j] as i32) * (b.elements[j] as i32)) as i32)
-                * (zeta as i32),
+        ai_bi + (aj_bj as i32)* (zeta as i32),
     );
+    hax_lib::fstar!("Spec.Utils.lemma_mul_i16b 3328 3328 (Seq.index (${a}.f_elements) (v i)) (Seq.index (${b}.f_elements) (v j))");
+    hax_lib::fstar!("Spec.Utils.lemma_mul_i16b 3328 3328 (Seq.index (${a}.f_elements) (v j)) (Seq.index (${b}.f_elements) (v i))");
     let o1 = montgomery_reduce_element(
         (a.elements[i] as i32) * (b.elements[j] as i32)
             + (a.elements[j] as i32) * (b.elements[i] as i32),
