libcrux-ml-kem/proofs/fstar/extraction/Libcrux_ml_kem.Vector.Portable.Ntt.fst
@@ -4,27 +4,27 @@ open Core
 open FStar.Mul
 
 let inv_ntt_step
-      (v: Libcrux_ml_kem.Vector.Portable.Vector_type.t_PortableVector)
+      (vec: Libcrux_ml_kem.Vector.Portable.Vector_type.t_PortableVector)
       (zeta: i16)
       (i j: usize)
      =
   let a_minus_b:i16 =
-    (v.Libcrux_ml_kem.Vector.Portable.Vector_type.f_elements.[ j ] <: i16) -!
-    (v.Libcrux_ml_kem.Vector.Portable.Vector_type.f_elements.[ i ] <: i16)
+    (vec.Libcrux_ml_kem.Vector.Portable.Vector_type.f_elements.[ j ] <: i16) -!
+    (vec.Libcrux_ml_kem.Vector.Portable.Vector_type.f_elements.[ i ] <: i16)
   in
-  let v:Libcrux_ml_kem.Vector.Portable.Vector_type.t_PortableVector =
+  let vec:Libcrux_ml_kem.Vector.Portable.Vector_type.t_PortableVector =
     {
-      v with
+      vec with
       Libcrux_ml_kem.Vector.Portable.Vector_type.f_elements
       =
-      Rust_primitives.Hax.Monomorphized_update_at.update_at_usize v
+      Rust_primitives.Hax.Monomorphized_update_at.update_at_usize vec
           .Libcrux_ml_kem.Vector.Portable.Vector_type.f_elements
         i
-        (Libcrux_ml_kem.Vector.Portable.Arithmetic.barrett_reduce_element ((v
+        (Libcrux_ml_kem.Vector.Portable.Arithmetic.barrett_reduce_element ((vec
                   .Libcrux_ml_kem.Vector.Portable.Vector_type.f_elements.[ i ]
                 <:
                 i16) +!
-              (v.Libcrux_ml_kem.Vector.Portable.Vector_type.f_elements.[ j ] <: i16)
+              (vec.Libcrux_ml_kem.Vector.Portable.Vector_type.f_elements.[ j ] <: i16)
               <:
               i16)
           <:
@@ -33,12 +33,12 @@ let inv_ntt_step
     <:
     Libcrux_ml_kem.Vector.Portable.Vector_type.t_PortableVector
   in
-  let v:Libcrux_ml_kem.Vector.Portable.Vector_type.t_PortableVector =
+  let vec:Libcrux_ml_kem.Vector.Portable.Vector_type.t_PortableVector =
     {
-      v with
+      vec with
       Libcrux_ml_kem.Vector.Portable.Vector_type.f_elements
       =
-      Rust_primitives.Hax.Monomorphized_update_at.update_at_usize v
+      Rust_primitives.Hax.Monomorphized_update_at.update_at_usize vec
           .Libcrux_ml_kem.Vector.Portable.Vector_type.f_elements
         j
         (Libcrux_ml_kem.Vector.Portable.Arithmetic.montgomery_multiply_fe_by_fer a_minus_b zeta
@@ -48,165 +48,167 @@ let inv_ntt_step
     <:
     Libcrux_ml_kem.Vector.Portable.Vector_type.t_PortableVector
   in
-  v
+  vec
 
 let inv_ntt_layer_1_step
-      (v: Libcrux_ml_kem.Vector.Portable.Vector_type.t_PortableVector)
+      (vec: Libcrux_ml_kem.Vector.Portable.Vector_type.t_PortableVector)
       (zeta0 zeta1 zeta2 zeta3: i16)
      =
-  let v:Libcrux_ml_kem.Vector.Portable.Vector_type.t_PortableVector =
-    inv_ntt_step v zeta0 (sz 0) (sz 2)
+  let vec:Libcrux_ml_kem.Vector.Portable.Vector_type.t_PortableVector =
+    inv_ntt_step vec zeta0 (sz 0) (sz 2)
   in
-  let v:Libcrux_ml_kem.Vector.Portable.Vector_type.t_PortableVector =
-    inv_ntt_step v zeta0 (sz 1) (sz 3)
+  let vec:Libcrux_ml_kem.Vector.Portable.Vector_type.t_PortableVector =
+    inv_ntt_step vec zeta0 (sz 1) (sz 3)
   in
-  let v:Libcrux_ml_kem.Vector.Portable.Vector_type.t_PortableVector =
-    inv_ntt_step v zeta1 (sz 4) (sz 6)
+  let vec:Libcrux_ml_kem.Vector.Portable.Vector_type.t_PortableVector =
+    inv_ntt_step vec zeta1 (sz 4) (sz 6)
   in
-  let v:Libcrux_ml_kem.Vector.Portable.Vector_type.t_PortableVector =
-    inv_ntt_step v zeta1 (sz 5) (sz 7)
+  let vec:Libcrux_ml_kem.Vector.Portable.Vector_type.t_PortableVector =
+    inv_ntt_step vec zeta1 (sz 5) (sz 7)
   in
-  let v:Libcrux_ml_kem.Vector.Portable.Vector_type.t_PortableVector =
-    inv_ntt_step v zeta2 (sz 8) (sz 10)
+  let vec:Libcrux_ml_kem.Vector.Portable.Vector_type.t_PortableVector =
+    inv_ntt_step vec zeta2 (sz 8) (sz 10)
   in
-  let v:Libcrux_ml_kem.Vector.Portable.Vector_type.t_PortableVector =
-    inv_ntt_step v zeta2 (sz 9) (sz 11)
+  let vec:Libcrux_ml_kem.Vector.Portable.Vector_type.t_PortableVector =
+    inv_ntt_step vec zeta2 (sz 9) (sz 11)
   in
-  let v:Libcrux_ml_kem.Vector.Portable.Vector_type.t_PortableVector =
-    inv_ntt_step v zeta3 (sz 12) (sz 14)
+  let vec:Libcrux_ml_kem.Vector.Portable.Vector_type.t_PortableVector =
+    inv_ntt_step vec zeta3 (sz 12) (sz 14)
   in
-  let v:Libcrux_ml_kem.Vector.Portable.Vector_type.t_PortableVector =
-    inv_ntt_step v zeta3 (sz 13) (sz 15)
+  let vec:Libcrux_ml_kem.Vector.Portable.Vector_type.t_PortableVector =
+    inv_ntt_step vec zeta3 (sz 13) (sz 15)
   in
-  v
+  vec
 
 let inv_ntt_layer_2_step
-      (v: Libcrux_ml_kem.Vector.Portable.Vector_type.t_PortableVector)
+      (vec: Libcrux_ml_kem.Vector.Portable.Vector_type.t_PortableVector)
       (zeta0 zeta1: i16)
      =
-  let v:Libcrux_ml_kem.Vector.Portable.Vector_type.t_PortableVector =
-    inv_ntt_step v zeta0 (sz 0) (sz 4)
+  let vec:Libcrux_ml_kem.Vector.Portable.Vector_type.t_PortableVector =
+    inv_ntt_step vec zeta0 (sz 0) (sz 4)
   in
-  let v:Libcrux_ml_kem.Vector.Portable.Vector_type.t_PortableVector =
-    inv_ntt_step v zeta0 (sz 1) (sz 5)
+  let vec:Libcrux_ml_kem.Vector.Portable.Vector_type.t_PortableVector =
+    inv_ntt_step vec zeta0 (sz 1) (sz 5)
   in
-  let v:Libcrux_ml_kem.Vector.Portable.Vector_type.t_PortableVector =
-    inv_ntt_step v zeta0 (sz 2) (sz 6)
+  let vec:Libcrux_ml_kem.Vector.Portable.Vector_type.t_PortableVector =
+    inv_ntt_step vec zeta0 (sz 2) (sz 6)
   in
-  let v:Libcrux_ml_kem.Vector.Portable.Vector_type.t_PortableVector =
-    inv_ntt_step v zeta0 (sz 3) (sz 7)
+  let vec:Libcrux_ml_kem.Vector.Portable.Vector_type.t_PortableVector =
+    inv_ntt_step vec zeta0 (sz 3) (sz 7)
   in
-  let v:Libcrux_ml_kem.Vector.Portable.Vector_type.t_PortableVector =
-    inv_ntt_step v zeta1 (sz 8) (sz 12)
+  let vec:Libcrux_ml_kem.Vector.Portable.Vector_type.t_PortableVector =
+    inv_ntt_step vec zeta1 (sz 8) (sz 12)
   in
-  let v:Libcrux_ml_kem.Vector.Portable.Vector_type.t_PortableVector =
-    inv_ntt_step v zeta1 (sz 9) (sz 13)
+  let vec:Libcrux_ml_kem.Vector.Portable.Vector_type.t_PortableVector =
+    inv_ntt_step vec zeta1 (sz 9) (sz 13)
   in
-  let v:Libcrux_ml_kem.Vector.Portable.Vector_type.t_PortableVector =
-    inv_ntt_step v zeta1 (sz 10) (sz 14)
+  let vec:Libcrux_ml_kem.Vector.Portable.Vector_type.t_PortableVector =
+    inv_ntt_step vec zeta1 (sz 10) (sz 14)
   in
-  let v:Libcrux_ml_kem.Vector.Portable.Vector_type.t_PortableVector =
-    inv_ntt_step v zeta1 (sz 11) (sz 15)
+  let vec:Libcrux_ml_kem.Vector.Portable.Vector_type.t_PortableVector =
+    inv_ntt_step vec zeta1 (sz 11) (sz 15)
   in
-  v
+  vec
 
 let inv_ntt_layer_3_step
-      (v: Libcrux_ml_kem.Vector.Portable.Vector_type.t_PortableVector)
+      (vec: Libcrux_ml_kem.Vector.Portable.Vector_type.t_PortableVector)
       (zeta: i16)
      =
-  let v:Libcrux_ml_kem.Vector.Portable.Vector_type.t_PortableVector =
-    inv_ntt_step v zeta (sz 0) (sz 8)
+  let vec:Libcrux_ml_kem.Vector.Portable.Vector_type.t_PortableVector =
+    inv_ntt_step vec zeta (sz 0) (sz 8)
   in
-  let v:Libcrux_ml_kem.Vector.Portable.Vector_type.t_PortableVector =
-    inv_ntt_step v zeta (sz 1) (sz 9)
+  let vec:Libcrux_ml_kem.Vector.Portable.Vector_type.t_PortableVector =
+    inv_ntt_step vec zeta (sz 1) (sz 9)
   in
-  let v:Libcrux_ml_kem.Vector.Portable.Vector_type.t_PortableVector =
-    inv_ntt_step v zeta (sz 2) (sz 10)
+  let vec:Libcrux_ml_kem.Vector.Portable.Vector_type.t_PortableVector =
+    inv_ntt_step vec zeta (sz 2) (sz 10)
   in
-  let v:Libcrux_ml_kem.Vector.Portable.Vector_type.t_PortableVector =
-    inv_ntt_step v zeta (sz 3) (sz 11)
+  let vec:Libcrux_ml_kem.Vector.Portable.Vector_type.t_PortableVector =
+    inv_ntt_step vec zeta (sz 3) (sz 11)
   in
-  let v:Libcrux_ml_kem.Vector.Portable.Vector_type.t_PortableVector =
-    inv_ntt_step v zeta (sz 4) (sz 12)
+  let vec:Libcrux_ml_kem.Vector.Portable.Vector_type.t_PortableVector =
+    inv_ntt_step vec zeta (sz 4) (sz 12)
   in
-  let v:Libcrux_ml_kem.Vector.Portable.Vector_type.t_PortableVector =
-    inv_ntt_step v zeta (sz 5) (sz 13)
+  let vec:Libcrux_ml_kem.Vector.Portable.Vector_type.t_PortableVector =
+    inv_ntt_step vec zeta (sz 5) (sz 13)
   in
-  let v:Libcrux_ml_kem.Vector.Portable.Vector_type.t_PortableVector =
-    inv_ntt_step v zeta (sz 6) (sz 14)
+  let vec:Libcrux_ml_kem.Vector.Portable.Vector_type.t_PortableVector =
+    inv_ntt_step vec zeta (sz 6) (sz 14)
   in
-  let v:Libcrux_ml_kem.Vector.Portable.Vector_type.t_PortableVector =
-    inv_ntt_step v zeta (sz 7) (sz 15)
+  let vec:Libcrux_ml_kem.Vector.Portable.Vector_type.t_PortableVector =
+    inv_ntt_step vec zeta (sz 7) (sz 15)
   in
-  v
+  vec
 
-let vu16 (b1:u16) : nat = 
-  let r = v b1 in
-  assert (r >= 0);
-  r
-  
-
-#push-options "--z3rlimit 150"
-val mul_i16b (b1 b2:u16) (n1 n2:i16):
-  Pure i32
-  (requires (let vb1: nat = v b1 in Spec.Utils.is_i16b vb1 n1))
-  (ensures (fun _ -> True))
-  
-  //z /\ Spec.Utils.is_i16b (v b2) n2))
-  (ensures (fun _ -> Spec.Utils.is_i32b (v b1 * v b2) ((cast n1 <: i32) *! (cast n2 <: i32))))
-
-let mul_i16b (b1 b2:u16) (n1 n2:i16) =
-
-#push-options "--z3rlimit 300 --query_stats --split_queries always"
 let ntt_multiply_binomials
       (a b: Libcrux_ml_kem.Vector.Portable.Vector_type.t_PortableVector)
       (zeta: i16)
       (i j: usize)
       (out: Libcrux_ml_kem.Vector.Portable.Vector_type.t_PortableVector)
      =
-  let ai = (cast (a
+  let _:Prims.unit =
+    Spec.Utils.lemma_mul_i16b 3328
+      3328
+      (Seq.index (a.f_elements) (v i))
+      (Seq.index (b.f_elements) (v i))
+  in
+  let _:Prims.unit =
+    Spec.Utils.lemma_mul_i16b 3328
+      3328
+      (Seq.index (a.f_elements) (v j))
+      (Seq.index (b.f_elements) (v j))
+  in
+  let ai_bi:i32 =
+    (cast (a.Libcrux_ml_kem.Vector.Portable.Vector_type.f_elements.[ i ] <: i16) <: i32) *!
+    (cast (b.Libcrux_ml_kem.Vector.Portable.Vector_type.f_elements.[ i ] <: i16) <: i32)
+  in
+  let aj_bj:i16 =
+    Libcrux_ml_kem.Vector.Portable.Arithmetic.montgomery_reduce_element ((cast (a
+                .Libcrux_ml_kem.Vector.Portable.Vector_type.f_elements.[ j ]
+              <:
+              i16)
+          <:
+          i32) *!
+        (cast (b.Libcrux_ml_kem.Vector.Portable.Vector_type.f_elements.[ j ] <: i16) <: i32)
+        <:
+        i32)
+  in
+  let _:Prims.unit = Spec.Utils.lemma_mul_i16b 3328 1664 aj_bj zeta in
+  let o0:i16 =
+    Libcrux_ml_kem.Vector.Portable.Arithmetic.montgomery_reduce_element (ai_bi +!
+        ((cast (aj_bj <: i16) <: i32) *! (cast (zeta <: i16) <: i32) <: i32)
+        <:
+        i32)
+  in
+  let _:Prims.unit =
+    Spec.Utils.lemma_mul_i16b 3328
+      3328
+      (Seq.index (a.f_elements) (v i))
+      (Seq.index (b.f_elements) (v j))
+  in
+  let _:Prims.unit =
+    Spec.Utils.lemma_mul_i16b 3328
+      3328
+      (Seq.index (a.f_elements) (v j))
+      (Seq.index (b.f_elements) (v i))
+  in
+  let o1:i16 =
+    Libcrux_ml_kem.Vector.Portable.Arithmetic.montgomery_reduce_element (((cast (a
                   .Libcrux_ml_kem.Vector.Portable.Vector_type.f_elements.[ i ]
                 <:
                 i16)
             <:
-            i32) in
-  assert (Spec.Utils.is_i32b 3328 ai);
-  let bi = (cast (b.Libcrux_ml_kem.Vector.Portable.Vector_type.f_elements.[ i ] <: i16) <: i32) in 
-  assert (Spec.Utils.is_i32b 3328 bi);
-  let aj = (cast (a
-                  .Libcrux_ml_kem.Vector.Portable.Vector_type.f_elements.[ j ]
-                <:
-                i16)
-            <:
-            i32) in
-  assert (Spec.Utils.is_i32b 3328 aj);
-  let bj = (cast (b.Libcrux_ml_kem.Vector.Portable.Vector_type.f_elements.[ j ] <: i16) <: i32) in 
-  assert (Spec.Utils.is_i32b 3328 bj);
-  Spec.Utils.lemma_mul_intb 3328 3328 (v ai) (v bi);
-  Spec.Utils.lemma_mul_intb 3328 3328 (v ai) (v bj);
-  Spec.Utils.lemma_mul_intb 3328 3328 (v aj) (v bi);
-  Spec.Utils.lemma_mul_intb 3328 3328 (v aj) (v bj);
-  let ai_bi = ai *! bi in
-  let aj_bj = Libcrux_ml_kem.Vector.Portable.Arithmetic.montgomery_reduce_element (aj *! bj) in
-  assert (Spec.Utils.is_i16b 3328 aj_bj);
-  Spec.Utils.lemma_mul_intb 3328 1664 (v aj_bj) (v zeta);
-  let aj_bj_zeta = (cast aj_bj <: i32) *. (cast (zeta <: i16) <: i32) in
-  assert (v aj_bj_zeta = v aj_bj * v zeta);
-  assert (Spec.Utils.is_i32b (3328 * 1664) aj_bj_zeta);
-  let sum = ai_bi +! aj_bj_zeta in
-  assert (Spec.Utils.is_i32b (3328 * 3328 + 3328 * 1664) sum);
-  let red = Libcrux_ml_kem.Vector.Portable.Arithmetic.montgomery_reduce_element sum in
-  assert (Spec.Utils.is_i16b (3328 + 1665) red);
-  Spec.Utils.lemma_mul_intb (3328 + 1665) 1664 (v red) (v zeta);
-  let mul = (cast red <: i32) *!  (cast (zeta <: i16) <: i32) in
-  let o0:i16 = Libcrux_ml_kem.Vector.Portable.Arithmetic.montgomery_reduce_element mul in
-  let ai_bj = ai *! bj in
-  let aj_bi = aj *! bi in
-  let sum = ai_bj +! aj_bi in
-  assert (Spec.Utils.is_i32b (2 * 3328 * 3328) sum);
-  let o1:i16 = Libcrux_ml_kem.Vector.Portable.Arithmetic.montgomery_reduce_element sum
+            i32) *!
+          (cast (b.Libcrux_ml_kem.Vector.Portable.Vector_type.f_elements.[ j ] <: i16) <: i32)
+          <:
+          i32) +!
+        ((cast (a.Libcrux_ml_kem.Vector.Portable.Vector_type.f_elements.[ j ] <: i16) <: i32) *!
+          (cast (b.Libcrux_ml_kem.Vector.Portable.Vector_type.f_elements.[ i ] <: i16) <: i32)
+          <:
+          i32)
+        <:
+        i32)
   in
-  admit()
   let out:Libcrux_ml_kem.Vector.Portable.Vector_type.t_PortableVector =
     {
       out with
@@ -236,131 +238,131 @@ let ntt_multiply_binomials
   out
 
 let ntt_step
-      (v: Libcrux_ml_kem.Vector.Portable.Vector_type.t_PortableVector)
+      (vec: Libcrux_ml_kem.Vector.Portable.Vector_type.t_PortableVector)
       (zeta: i16)
       (i j: usize)
      =
   let t:i16 =
-    Libcrux_ml_kem.Vector.Portable.Arithmetic.montgomery_multiply_fe_by_fer (v
+    Libcrux_ml_kem.Vector.Portable.Arithmetic.montgomery_multiply_fe_by_fer (vec
           .Libcrux_ml_kem.Vector.Portable.Vector_type.f_elements.[ j ]
         <:
         i16)
       zeta
   in
-  let v:Libcrux_ml_kem.Vector.Portable.Vector_type.t_PortableVector =
+  let vec:Libcrux_ml_kem.Vector.Portable.Vector_type.t_PortableVector =
     {
-      v with
+      vec with
       Libcrux_ml_kem.Vector.Portable.Vector_type.f_elements
       =
-      Rust_primitives.Hax.Monomorphized_update_at.update_at_usize v
+      Rust_primitives.Hax.Monomorphized_update_at.update_at_usize vec
           .Libcrux_ml_kem.Vector.Portable.Vector_type.f_elements
         j
-        ((v.Libcrux_ml_kem.Vector.Portable.Vector_type.f_elements.[ i ] <: i16) -! t <: i16)
+        ((vec.Libcrux_ml_kem.Vector.Portable.Vector_type.f_elements.[ i ] <: i16) -! t <: i16)
     }
     <:
     Libcrux_ml_kem.Vector.Portable.Vector_type.t_PortableVector
   in
-  let v:Libcrux_ml_kem.Vector.Portable.Vector_type.t_PortableVector =
+  let vec:Libcrux_ml_kem.Vector.Portable.Vector_type.t_PortableVector =
     {
-      v with
+      vec with
       Libcrux_ml_kem.Vector.Portable.Vector_type.f_elements
       =
-      Rust_primitives.Hax.Monomorphized_update_at.update_at_usize v
+      Rust_primitives.Hax.Monomorphized_update_at.update_at_usize vec
           .Libcrux_ml_kem.Vector.Portable.Vector_type.f_elements
         i
-        ((v.Libcrux_ml_kem.Vector.Portable.Vector_type.f_elements.[ i ] <: i16) +! t <: i16)
+        ((vec.Libcrux_ml_kem.Vector.Portable.Vector_type.f_elements.[ i ] <: i16) +! t <: i16)
     }
     <:
     Libcrux_ml_kem.Vector.Portable.Vector_type.t_PortableVector
   in
-  v
+  vec
 
 let ntt_layer_1_step
-      (v: Libcrux_ml_kem.Vector.Portable.Vector_type.t_PortableVector)
+      (vec: Libcrux_ml_kem.Vector.Portable.Vector_type.t_PortableVector)
       (zeta0 zeta1 zeta2 zeta3: i16)
      =
-  let v:Libcrux_ml_kem.Vector.Portable.Vector_type.t_PortableVector =
-    ntt_step v zeta0 (sz 0) (sz 2)
+  let vec:Libcrux_ml_kem.Vector.Portable.Vector_type.t_PortableVector =
+    ntt_step vec zeta0 (sz 0) (sz 2)
   in
-  let v:Libcrux_ml_kem.Vector.Portable.Vector_type.t_PortableVector =
-    ntt_step v zeta0 (sz 1) (sz 3)
+  let vec:Libcrux_ml_kem.Vector.Portable.Vector_type.t_PortableVector =
+    ntt_step vec zeta0 (sz 1) (sz 3)
   in
-  let v:Libcrux_ml_kem.Vector.Portable.Vector_type.t_PortableVector =
-    ntt_step v zeta1 (sz 4) (sz 6)
+  let vec:Libcrux_ml_kem.Vector.Portable.Vector_type.t_PortableVector =
+    ntt_step vec zeta1 (sz 4) (sz 6)
   in
-  let v:Libcrux_ml_kem.Vector.Portable.Vector_type.t_PortableVector =
-    ntt_step v zeta1 (sz 5) (sz 7)
+  let vec:Libcrux_ml_kem.Vector.Portable.Vector_type.t_PortableVector =
+    ntt_step vec zeta1 (sz 5) (sz 7)
   in
-  let v:Libcrux_ml_kem.Vector.Portable.Vector_type.t_PortableVector =
-    ntt_step v zeta2 (sz 8) (sz 10)
+  let vec:Libcrux_ml_kem.Vector.Portable.Vector_type.t_PortableVector =
+    ntt_step vec zeta2 (sz 8) (sz 10)
   in
-  let v:Libcrux_ml_kem.Vector.Portable.Vector_type.t_PortableVector =
-    ntt_step v zeta2 (sz 9) (sz 11)
+  let vec:Libcrux_ml_kem.Vector.Portable.Vector_type.t_PortableVector =
+    ntt_step vec zeta2 (sz 9) (sz 11)
   in
-  let v:Libcrux_ml_kem.Vector.Portable.Vector_type.t_PortableVector =
-    ntt_step v zeta3 (sz 12) (sz 14)
+  let vec:Libcrux_ml_kem.Vector.Portable.Vector_type.t_PortableVector =
+    ntt_step vec zeta3 (sz 12) (sz 14)
   in
-  let v:Libcrux_ml_kem.Vector.Portable.Vector_type.t_PortableVector =
-    ntt_step v zeta3 (sz 13) (sz 15)
+  let vec:Libcrux_ml_kem.Vector.Portable.Vector_type.t_PortableVector =
+    ntt_step vec zeta3 (sz 13) (sz 15)
   in
-  v
+  vec
 
 let ntt_layer_2_step
-      (v: Libcrux_ml_kem.Vector.Portable.Vector_type.t_PortableVector)
+      (vec: Libcrux_ml_kem.Vector.Portable.Vector_type.t_PortableVector)
       (zeta0 zeta1: i16)
      =
-  let v:Libcrux_ml_kem.Vector.Portable.Vector_type.t_PortableVector =
-    ntt_step v zeta0 (sz 0) (sz 4)
+  let vec:Libcrux_ml_kem.Vector.Portable.Vector_type.t_PortableVector =
+    ntt_step vec zeta0 (sz 0) (sz 4)
   in
-  let v:Libcrux_ml_kem.Vector.Portable.Vector_type.t_PortableVector =
-    ntt_step v zeta0 (sz 1) (sz 5)
+  let vec:Libcrux_ml_kem.Vector.Portable.Vector_type.t_PortableVector =
+    ntt_step vec zeta0 (sz 1) (sz 5)
   in
-  let v:Libcrux_ml_kem.Vector.Portable.Vector_type.t_PortableVector =
-    ntt_step v zeta0 (sz 2) (sz 6)
+  let vec:Libcrux_ml_kem.Vector.Portable.Vector_type.t_PortableVector =
+    ntt_step vec zeta0 (sz 2) (sz 6)
   in
-  let v:Libcrux_ml_kem.Vector.Portable.Vector_type.t_PortableVector =
-    ntt_step v zeta0 (sz 3) (sz 7)
+  let vec:Libcrux_ml_kem.Vector.Portable.Vector_type.t_PortableVector =
+    ntt_step vec zeta0 (sz 3) (sz 7)
   in
-  let v:Libcrux_ml_kem.Vector.Portable.Vector_type.t_PortableVector =
-    ntt_step v zeta1 (sz 8) (sz 12)
+  let vec:Libcrux_ml_kem.Vector.Portable.Vector_type.t_PortableVector =
+    ntt_step vec zeta1 (sz 8) (sz 12)
   in
-  let v:Libcrux_ml_kem.Vector.Portable.Vector_type.t_PortableVector =
-    ntt_step v zeta1 (sz 9) (sz 13)
+  let vec:Libcrux_ml_kem.Vector.Portable.Vector_type.t_PortableVector =
+    ntt_step vec zeta1 (sz 9) (sz 13)
   in
-  let v:Libcrux_ml_kem.Vector.Portable.Vector_type.t_PortableVector =
-    ntt_step v zeta1 (sz 10) (sz 14)
+  let vec:Libcrux_ml_kem.Vector.Portable.Vector_type.t_PortableVector =
+    ntt_step vec zeta1 (sz 10) (sz 14)
   in
-  let v:Libcrux_ml_kem.Vector.Portable.Vector_type.t_PortableVector =
-    ntt_step v zeta1 (sz 11) (sz 15)
+  let vec:Libcrux_ml_kem.Vector.Portable.Vector_type.t_PortableVector =
+    ntt_step vec zeta1 (sz 11) (sz 15)
   in
-  v
+  vec
 
-let ntt_layer_3_step (v: Libcrux_ml_kem.Vector.Portable.Vector_type.t_PortableVector) (zeta: i16) =
-  let v:Libcrux_ml_kem.Vector.Portable.Vector_type.t_PortableVector =
-    ntt_step v zeta (sz 0) (sz 8)
+let ntt_layer_3_step (vec: Libcrux_ml_kem.Vector.Portable.Vector_type.t_PortableVector) (zeta: i16) =
+  let vec:Libcrux_ml_kem.Vector.Portable.Vector_type.t_PortableVector =
+    ntt_step vec zeta (sz 0) (sz 8)
   in
-  let v:Libcrux_ml_kem.Vector.Portable.Vector_type.t_PortableVector =
-    ntt_step v zeta (sz 1) (sz 9)
+  let vec:Libcrux_ml_kem.Vector.Portable.Vector_type.t_PortableVector =
+    ntt_step vec zeta (sz 1) (sz 9)
   in
-  let v:Libcrux_ml_kem.Vector.Portable.Vector_type.t_PortableVector =
-    ntt_step v zeta (sz 2) (sz 10)
+  let vec:Libcrux_ml_kem.Vector.Portable.Vector_type.t_PortableVector =
+    ntt_step vec zeta (sz 2) (sz 10)
   in
-  let v:Libcrux_ml_kem.Vector.Portable.Vector_type.t_PortableVector =
-    ntt_step v zeta (sz 3) (sz 11)
+  let vec:Libcrux_ml_kem.Vector.Portable.Vector_type.t_PortableVector =
+    ntt_step vec zeta (sz 3) (sz 11)
   in
-  let v:Libcrux_ml_kem.Vector.Portable.Vector_type.t_PortableVector =
-    ntt_step v zeta (sz 4) (sz 12)
+  let vec:Libcrux_ml_kem.Vector.Portable.Vector_type.t_PortableVector =
+    ntt_step vec zeta (sz 4) (sz 12)
   in
-  let v:Libcrux_ml_kem.Vector.Portable.Vector_type.t_PortableVector =
-    ntt_step v zeta (sz 5) (sz 13)
+  let vec:Libcrux_ml_kem.Vector.Portable.Vector_type.t_PortableVector =
+    ntt_step vec zeta (sz 5) (sz 13)
   in
-  let v:Libcrux_ml_kem.Vector.Portable.Vector_type.t_PortableVector =
-    ntt_step v zeta (sz 6) (sz 14)
+  let vec:Libcrux_ml_kem.Vector.Portable.Vector_type.t_PortableVector =
+    ntt_step vec zeta (sz 6) (sz 14)
   in
-  let v:Libcrux_ml_kem.Vector.Portable.Vector_type.t_PortableVector =
-    ntt_step v zeta (sz 7) (sz 15)
+  let vec:Libcrux_ml_kem.Vector.Portable.Vector_type.t_PortableVector =
+    ntt_step vec zeta (sz 7) (sz 15)
   in
-  v
+  vec
 
 let ntt_multiply
       (lhs rhs: Libcrux_ml_kem.Vector.Portable.Vector_type.t_PortableVector)
