libcrux-ml-kem/proofs/fstar/extraction/Libcrux_ml_kem.Vector.Avx2.fsti
@@ -58,24 +58,24 @@ let impl_3: Libcrux_ml_kem.Vector.Traits.t_Operations t_SIMD256Vector =
     f_ZERO_pre = (fun (_: Prims.unit) -> true);
     f_ZERO_post
     =
-    (fun (_: Prims.unit) (out: t_SIMD256Vector) -> impl.f_repr out == Seq.create 16 0s);
+    (fun (_: Prims.unit) (result: t_SIMD256Vector) -> impl.f_repr out == Seq.create 16 0s);
     f_ZERO = (fun (_: Prims.unit) -> vec_zero ());
     f_from_i16_array_pre
     =
     (fun (array: t_Slice i16) -> (Core.Slice.impl__len #i16 array <: usize) =. sz 16);
     f_from_i16_array_post
     =
-    (fun (array: t_Slice i16) (out: t_SIMD256Vector) -> impl.f_repr out == array);
+    (fun (array: t_Slice i16) (result: t_SIMD256Vector) -> impl.f_repr out == array);
     f_from_i16_array = (fun (array: t_Slice i16) -> vec_from_i16_array array);
     f_to_i16_array_pre = (fun (x: t_SIMD256Vector) -> true);
     f_to_i16_array_post
     =
-    (fun (x: t_SIMD256Vector) (out: t_Array i16 (sz 16)) -> out == impl.f_repr x);
+    (fun (x: t_SIMD256Vector) (result: t_Array i16 (sz 16)) -> out == impl.f_repr x);
     f_to_i16_array = (fun (x: t_SIMD256Vector) -> vec_to_i16_array x);
     f_add_pre = (fun (lhs: t_SIMD256Vector) (rhs: t_SIMD256Vector) -> true);
     f_add_post
     =
-    (fun (lhs: t_SIMD256Vector) (rhs: t_SIMD256Vector) (out: t_SIMD256Vector) ->
+    (fun (lhs: t_SIMD256Vector) (rhs: t_SIMD256Vector) (result: t_SIMD256Vector) ->
         impl.f_repr out == Spec.Utils.map2 ( +. ) (impl.f_repr lhs) (impl.f_repr rhs));
     f_add
     =
@@ -86,7 +86,7 @@ let impl_3: Libcrux_ml_kem.Vector.Traits.t_Operations t_SIMD256Vector =
     f_sub_pre = (fun (lhs: t_SIMD256Vector) (rhs: t_SIMD256Vector) -> true);
     f_sub_post
     =
-    (fun (lhs: t_SIMD256Vector) (rhs: t_SIMD256Vector) (out: t_SIMD256Vector) ->
+    (fun (lhs: t_SIMD256Vector) (rhs: t_SIMD256Vector) (result: t_SIMD256Vector) ->
         impl.f_repr out == Spec.Utils.map2 ( -. ) (impl.f_repr lhs) (impl.f_repr rhs));
     f_sub
     =
@@ -97,7 +97,7 @@ let impl_3: Libcrux_ml_kem.Vector.Traits.t_Operations t_SIMD256Vector =
     f_multiply_by_constant_pre = (fun (v: t_SIMD256Vector) (c: i16) -> true);
     f_multiply_by_constant_post
     =
-    (fun (v: t_SIMD256Vector) (c: i16) (out: t_SIMD256Vector) ->
+    (fun (v: t_SIMD256Vector) (c: i16) (result: t_SIMD256Vector) ->
         impl.f_repr out == Spec.Utils.map_array (fun x -> x *. c) (impl.f_repr v));
     f_multiply_by_constant
     =
@@ -108,7 +108,7 @@ let impl_3: Libcrux_ml_kem.Vector.Traits.t_Operations t_SIMD256Vector =
     f_bitwise_and_with_constant_pre = (fun (vector: t_SIMD256Vector) (constant: i16) -> true);
     f_bitwise_and_with_constant_post
     =
-    (fun (vector: t_SIMD256Vector) (constant: i16) (out: t_SIMD256Vector) ->
+    (fun (vector: t_SIMD256Vector) (constant: i16) (result: t_SIMD256Vector) ->
         impl.f_repr out == Spec.Utils.map_array (fun x -> x &. constant) (impl.f_repr vector));
     f_bitwise_and_with_constant
     =
@@ -125,7 +125,7 @@ let impl_3: Libcrux_ml_kem.Vector.Traits.t_Operations t_SIMD256Vector =
     (fun (v_SHIFT_BY: i32) (vector: t_SIMD256Vector) -> v_SHIFT_BY >=. 0l && v_SHIFT_BY <. 16l);
     f_shift_right_post
     =
-    (fun (v_SHIFT_BY: i32) (vector: t_SIMD256Vector) (out: t_SIMD256Vector) ->
+    (fun (v_SHIFT_BY: i32) (vector: t_SIMD256Vector) (result: t_SIMD256Vector) ->
         (v_SHIFT_BY >=. 0l /\ v_SHIFT_BY <. 16l) ==>
         impl.f_repr out == Spec.Utils.map_array (fun x -> x >>! v_SHIFT_BY) (impl.f_repr vector));
     f_shift_right
@@ -143,7 +143,7 @@ let impl_3: Libcrux_ml_kem.Vector.Traits.t_Operations t_SIMD256Vector =
     (fun (vector: t_SIMD256Vector) -> Spec.Utils.is_i16b_array (pow2 12 - 1) (impl.f_repr vector));
     f_cond_subtract_3329_post
     =
-    (fun (vector: t_SIMD256Vector) (out: t_SIMD256Vector) ->
+    (fun (vector: t_SIMD256Vector) (result: t_SIMD256Vector) ->
         impl.f_repr out ==
         Spec.Utils.map_array (fun x -> if x >=. 3329s then x -! 3329s else x) (impl.f_repr vector));
     f_cond_subtract_3329_
