libcrux-ml-kem/proofs/fstar/extraction/Libcrux_ml_kem.Vector.Portable.Ntt.fsti
@@ -4,32 +4,34 @@ open Core
 open FStar.Mul
 
 val inv_ntt_step
-      (v: Libcrux_ml_kem.Vector.Portable.Vector_type.t_PortableVector)
+      (vec: Libcrux_ml_kem.Vector.Portable.Vector_type.t_PortableVector)
       (zeta: i16)
       (i j: usize)
     : Prims.Pure Libcrux_ml_kem.Vector.Portable.Vector_type.t_PortableVector
-      Prims.l_True
+      (requires v i < 16 /\ v j < 16 /\ Spec.Utils.is_i16b 1664 zeta)
       (fun _ -> Prims.l_True)
 
 val inv_ntt_layer_1_step
-      (v: Libcrux_ml_kem.Vector.Portable.Vector_type.t_PortableVector)
+      (vec: Libcrux_ml_kem.Vector.Portable.Vector_type.t_PortableVector)
       (zeta0 zeta1 zeta2 zeta3: i16)
     : Prims.Pure Libcrux_ml_kem.Vector.Portable.Vector_type.t_PortableVector
-      Prims.l_True
+      (requires
+        Spec.Utils.is_i16b 1664 zeta0 /\ Spec.Utils.is_i16b 1664 zeta1 /\
+        Spec.Utils.is_i16b 1664 zeta2 /\ Spec.Utils.is_i16b 1664 zeta3)
       (fun _ -> Prims.l_True)
 
 val inv_ntt_layer_2_step
-      (v: Libcrux_ml_kem.Vector.Portable.Vector_type.t_PortableVector)
+      (vec: Libcrux_ml_kem.Vector.Portable.Vector_type.t_PortableVector)
       (zeta0 zeta1: i16)
     : Prims.Pure Libcrux_ml_kem.Vector.Portable.Vector_type.t_PortableVector
-      Prims.l_True
+      (requires Spec.Utils.is_i16b 1664 zeta0 /\ Spec.Utils.is_i16b 1664 zeta1)
       (fun _ -> Prims.l_True)
 
 val inv_ntt_layer_3_step
-      (v: Libcrux_ml_kem.Vector.Portable.Vector_type.t_PortableVector)
+      (vec: Libcrux_ml_kem.Vector.Portable.Vector_type.t_PortableVector)
       (zeta: i16)
     : Prims.Pure Libcrux_ml_kem.Vector.Portable.Vector_type.t_PortableVector
-      Prims.l_True
+      (requires Spec.Utils.is_i16b 1664 zeta)
       (fun _ -> Prims.l_True)
 
 /// Compute the product of two Kyber binomials with respect to the
@@ -54,48 +56,47 @@ val ntt_multiply_binomials
       (i j: usize)
       (out: Libcrux_ml_kem.Vector.Portable.Vector_type.t_PortableVector)
     : Prims.Pure Libcrux_ml_kem.Vector.Portable.Vector_type.t_PortableVector
-      (requires (v i < 16 /\ v j < 16 /\
-                 Spec.Utils.is_i16b_array 3328 a.f_elements /\
-                 Spec.Utils.is_i16b_array 3328 b.f_elements /\
-                 Spec.Utils.is_i16b 1664 zeta))
+      (requires v i < 16 /\ v j < 16 /\ Spec.Utils.is_i16b 1664 zeta)
       (ensures
         fun out_future ->
           let out_future:Libcrux_ml_kem.Vector.Portable.Vector_type.t_PortableVector = out_future in
-          let (x,y) =
-          Spec.MLKEM.Math.poly_base_case_multiply 
-            (v (Seq.index a.f_elements (v i)) % 3329)
-            (v (Seq.index a.f_elements (v j)) % 3329)
-            (v (Seq.index b.f_elements (v i)) % 3329)
-            (v (Seq.index b.f_elements (v j)) % 3329)
-            ((v zeta * 169) % 3329) in
+          let x, y =
+            Spec.MLKEM.Math.poly_base_case_multiply (v (Seq.index a.f_elements (v i)) % 3329)
+              (v (Seq.index a.f_elements (v j)) % 3329)
+              (v (Seq.index b.f_elements (v i)) % 3329)
+              (v (Seq.index b.f_elements (v j)) % 3329)
+              ((v zeta * 169) % 3329)
+          in
           (x == v (Seq.index out_future.f_elements (v i)) % 3329 /\
-           y == v (Seq.index out_future.f_elements (v j)) % 3329))
+            y == v (Seq.index out_future.f_elements (v j)) % 3329))
 
 val ntt_step
-      (v: Libcrux_ml_kem.Vector.Portable.Vector_type.t_PortableVector)
+      (vec: Libcrux_ml_kem.Vector.Portable.Vector_type.t_PortableVector)
       (zeta: i16)
       (i j: usize)
     : Prims.Pure Libcrux_ml_kem.Vector.Portable.Vector_type.t_PortableVector
-      Prims.l_True
+      (requires v i < 16 /\ v j < 16 /\ Spec.Utils.is_i16b 1664 zeta)
       (fun _ -> Prims.l_True)
 
 val ntt_layer_1_step
-      (v: Libcrux_ml_kem.Vector.Portable.Vector_type.t_PortableVector)
+      (vec: Libcrux_ml_kem.Vector.Portable.Vector_type.t_PortableVector)
       (zeta0 zeta1 zeta2 zeta3: i16)
     : Prims.Pure Libcrux_ml_kem.Vector.Portable.Vector_type.t_PortableVector
-      Prims.l_True
+      (requires
+        Spec.Utils.is_i16b 1664 zeta0 /\ Spec.Utils.is_i16b 1664 zeta1 /\
+        Spec.Utils.is_i16b 1664 zeta2 /\ Spec.Utils.is_i16b 1664 zeta3)
       (fun _ -> Prims.l_True)
 
 val ntt_layer_2_step
-      (v: Libcrux_ml_kem.Vector.Portable.Vector_type.t_PortableVector)
+      (vec: Libcrux_ml_kem.Vector.Portable.Vector_type.t_PortableVector)
       (zeta0 zeta1: i16)
     : Prims.Pure Libcrux_ml_kem.Vector.Portable.Vector_type.t_PortableVector
-      Prims.l_True
+      (requires Spec.Utils.is_i16b 1664 zeta0 /\ Spec.Utils.is_i16b 1664 zeta1)
       (fun _ -> Prims.l_True)
 
-val ntt_layer_3_step (v: Libcrux_ml_kem.Vector.Portable.Vector_type.t_PortableVector) (zeta: i16)
+val ntt_layer_3_step (vec: Libcrux_ml_kem.Vector.Portable.Vector_type.t_PortableVector) (zeta: i16)
     : Prims.Pure Libcrux_ml_kem.Vector.Portable.Vector_type.t_PortableVector
-      Prims.l_True
+      (requires Spec.Utils.is_i16b 1664 zeta)
       (fun _ -> Prims.l_True)
 
 val ntt_multiply
