libcrux-ml-kem/proofs/fstar/spec/Spec.Utils.fst
@@ -163,9 +163,12 @@ let lemma_at_percent_mod (v:int) (p:int{p>0/\ p%2=0}):
 
 let lemma_div_at_percent (v:int) (p:int{p>0/\ p%2=0 /\ (v/p) < p/2 /\ (v/p) >= -p / 2}):
   Lemma ((v / p) @% p == v / p) = 
-    assert ((v / p) < p);
-    assert ((v / p) @% p == v / p);
-    ()
+    let m = (v / p) % p in
+    if m >= p/2 then(
+      assert ((v/p) < 0);
+      assert (m - p == v/p)
+    )
+    else ()
 
 #push-options "--z3rlimit 1200 --split_queries always"
 val lemma_mont_red_i32 (x:i32): Lemma
